\chapter{Convolutions and Conditional expectation}

\section{Convolutions}

\begin{framed}
   \textbf{Theorem} [Discrete] Let $X, Y$ be independent r.v.s, the PMF of $T = X + Y$ is 
   \[
      P(T = t) =  \sum_{x} P(Y = t - x) \cdot P(X = x)
   \] 

   \textbf{Justification}: Law of Total Probability
   \[
      \text{LOTP}: P(B) = \sum_{i}P(B | A_i) P(A_i)
   \] 

   In this case
   \begin{align*}
      P(T = t) &= P(X + Y = t) \text{ by definition} \\
               &= \sum_{x} P( X + Y = t | X = x) \cdot P(X = x)  \text{ LOTP} \\
               &= \sum_{x}P( Y = t - x | X = x) \cdot P( X = x)  \text{ by rearranging}\\
               &= \sum_{x}P( Y = t - x ) \cdot P( X = x) \text{ by independence of $X, Y$}\\ 
   \end{align*}
\end{framed}

\begin{framed}
   \textbf{Theorem} [Continuous] Let $X, Y$ be independent r.v.s, the PDF of $T = X + Y$ is
    \[
     f_T(t) = \int_{\infty}^{\infty}  f_X(x) \cdot f_Y(t - x) dx 
   \] 
  
\end{framed}

